change computer to record

theories/ops.v
@@ -1,71 +1,100 @@
 From coq_sortscan Require Import helper.
 From stdpp Require Import list.
 
-Implicit Types disk mem : list nat.
+Definition CAP_DISK : nat := 100.
+Definition CAP_MEM : nat := 16.
 
-Definition write_const_disk disk mem (i v : nat) := <[i := v]> disk.
-Definition write_const_mem disk mem (i v : nat) := <[i := v]> mem.
-Definition read_mem disk mem (i : nat) := mem !! i.
+Record Data := {
+  disk : list nat;
+  mem : list nat;
+  disk_length : length disk = CAP_DISK;
+  mem_length : length mem = CAP_MEM
+}.
+
+Implicit Type (data : Data).
+
+Program Definition write_const_disk data (i v : nat) : Data :=
+  {| disk := <[i:=v]> (disk data); mem := mem data |}.
+Next Obligation. intros. rewrite insert_length. apply (disk_length data). Qed.
+Next Obligation. intros. apply (mem_length data). Qed.
+
+Program Definition write_const_mem data (i v : nat) : Data :=
+  {| disk := disk data; mem := <[i:=v]> (mem data) |}.
+Next Obligation. intros. apply (disk_length data). Qed.
+Next Obligation. intros. rewrite insert_length. apply (mem_length data). Qed.
+
+Definition read_mem data (i : nat) := (mem data) !! i.
 
 (* copy disk[i] to mem[j] *)
-Definition read_disk disk mem (i j : nat) :=
-  match disk !! i with
-  | None => mem
-  | Some v => write_const_mem disk mem j v
+Definition read_disk data (i j : nat) :=
+  match (disk data) !! i with
+  | None => data
+  | Some v => write_const_mem data j v
   end.
 
 (* copy mem[i] to disk[j] *)
-Definition write_disk disk mem (i j : nat) :=
-  read_disk mem disk i j.
+Definition write_disk data (i j : nat) :=
+  match (mem data) !! i with
+  | None => data
+  | Some v => write_const_disk data j v
+  end.
 
 (* copy disk[i..i+len) to mem[j..j+len) *)
-Fixpoint read_range_disk disk mem (i len j : nat) :=
+Fixpoint read_range_disk data (i len j : nat) :=
   match len with
-  | O => mem
-  | S len' => read_range_disk
-      disk (read_disk disk mem i j) (S i) len' (S j)
+  | O => data
+  | S len' => read_range_disk (read_disk data i j) (S i) len' (S j)
   end.
 
 (* copy mem[i..i+len) to disk[j..j+len) *)
-Definition write_range_disk disk mem (i len j : nat) :=
-  read_range_disk mem disk i len j.
-
-Lemma read_disk_length disk mem i j :
-  length (read_disk disk mem i j) = length mem.
+Fixpoint write_range_disk data (i len j : nat) :=
+  match len with
+  | O => data
+  | S len' => write_range_disk (write_disk data i j) (S i) len' (S j)
+  end.
+(*
+Lemma read_disk_length data i j :
+  length (read_disk data i j) = length mem.
 Proof.
   unfold read_disk. destruct (disk !! i) eqn:E; auto.
   unfold write_const_mem. by rewrite insert_length.
 Qed.
 
-Lemma read_range_disk_length disk mem i len j :
-  length (read_range_disk disk mem i len j) = length mem.
+Lemma read_range_disk_length data i len j :
+  length (read_range_disk data i len j) = length mem.
 Proof.
-  revert disk mem i j. induction len; auto; simpl; intros.
+  revert data i j. induction len; auto; simpl; intros.
   rewrite IHlen. by rewrite read_disk_length.
 Qed.
-
-Lemma read_range_disk_slice disk mem i len j :
-  slice (read_range_disk disk mem i len j) j len =
-  slice disk i len.
+*)
+Lemma read_range_disk_slice data i len j :
+  slice (mem (read_range_disk data i len j)) j len =
+  slice (disk data) i len.
 Admitted.
 
-Lemma read_range_disk_eq disk mem i len j :
-  read_range_disk disk mem i len j =
-  take j mem ++ slice disk i len ++ drop (j+len) mem.
+Lemma read_range_disk_eq data i len j :
+  mem (read_range_disk data i len j) =
+  take j (mem data) ++ slice (disk data) i len ++ drop (j+len) (mem data).
 Proof.
-  rewrite (slice_cut
-    (read_range_disk disk mem i len j) j len
-  ).
+  rewrite (slice_cut (mem (read_range_disk data i len j)) j len).
   rewrite read_range_disk_slice.
 Admitted.
-  (*
-Lemma read_disk_lookup disk mem i j :
-  i < length disk → j < length mem →
-  (read_disk disk mem i j) !! j = disk !! i.
+
+Lemma read_range_disk_disk data i len j :
+  disk (read_range_disk data i len j) = disk data.
 Admitted.
-*)
-Lemma write_range_disk_lookup disk mem i len j :
-  i+len ≤ length mem → j+len ≤ length disk →
-  slice (write_range_disk disk mem i len j) j len =
-  slice mem i len.
+
+Lemma write_range_disk_slice data i len j :
+  i+len ≤ CAP_MEM → j+len ≤ CAP_DISK →
+  slice (disk (write_range_disk data i len j)) j len =
+  slice (mem data) i len.
+Admitted.
+
+Lemma write_range_disk_eq data i len j :
+  disk (write_range_disk data i len j) =
+  take j (disk data) ++ slice (mem data) i len ++ drop (j+len) (disk data).
+Admitted.
+
+Lemma write_range_disk_mem data i len j :
+  mem (write_range_disk data i len j) = mem data.
 Admitted.
